venom/analysis/dataflow/proofs/dfHelperProofsScript.sml
@@ -4,7 +4,7 @@
 
 Theory dfHelperProofs
 Ancestors
-  dfHelperDefs pred_set
+  dfHelperDefs pred_set list
 
 Theorem list_intersect_set_proof:
   !xs ys. set (list_intersect xs ys) = set xs INTER set ys
@@ -29,4 +29,19 @@ Theorem list_intersect_all_mono_proof:
   !l ls. set (list_intersect_all (l :: ls)) SUBSET set l
 Proof
   cheat
+QED
+
+(* list_union: membership iff member of either list *)
+Theorem list_union_mem_proof:
+  !v xs ys. MEM v (list_union xs ys) <=> MEM v xs \/ MEM v ys
+Proof
+  rw[list_union_def, MEM_APPEND, MEM_FILTER] >> metis_tac[]
+QED
+
+(* list_union: set semantics *)
+Theorem list_union_set_proof:
+  !xs ys. set (list_union xs ys) = set xs UNION set ys
+Proof
+  rw[list_union_def, LIST_TO_SET_APPEND, LIST_TO_SET_FILTER, EXTENSION] >>
+  rw[MEM_FILTER] >> metis_tac[]
 QED
